

eepipi-tutorial

December 18, 2019

```
[1]: from sympy import *
```

```
[2]: import heppackv0 as hep
```

Reading heppackv0.py

Done

```
[3]: M,m,theta,phi, alpha=symbols('M m theta phi alpha',real=True)
t,t0,s,s0,p=symbols('t t0,s,s0,p',real=True)
E,P,beta,xi=symbols('E P beta xi',positive=True)
```

This tutorial will be less verbose than eemmuu.ipynb. Because the amplitudes are very simple we can afford to include a possible ϕ dependence right from the beginning.

```
[4]: pin=[E,m,0,0]
ki=[E,m,pi,pi]
pf=[E,M,theta,phi]
kf=[E,M,pi-theta,pi+phi]
```

```
[5]: pf4=simplify(hep.fourvec(pf));pf4
```

[5]:

$$\left[E, \quad 2\sqrt{E^2 - M^2} \sin\left(\frac{\theta}{2}\right) \cos(\phi) \cos\left(\frac{\theta}{2}\right), \quad 2\sqrt{E^2 - M^2} \sin(\phi) \sin\left(\frac{\theta}{2}\right) \cos\left(\frac{\theta}{2}\right), \quad \sqrt{E^2 - M^2} \left(-\sin^2\left(\frac{\theta}{2}\right) + \cos^2(\phi)\right) \right]$$

```
[6]: kf4=hep.fourvec(kf);kf4
```

[6]:

$$\left[E, \quad -2\sqrt{E^2 - M^2} \sin\left(\frac{\theta}{2}\right) \cos(\phi) \cos\left(\frac{\theta}{2}\right), \quad -2\sqrt{E^2 - M^2} \sin(\phi) \sin\left(\frac{\theta}{2}\right) \cos\left(\frac{\theta}{2}\right), \quad \sqrt{E^2 - M^2} \left(\sin^2\left(\frac{\theta}{2}\right) + \cos^2(\phi)\right) \right]$$

The Feynman rules require $p_f^\mu - k_f^\mu$ at the outgoing vertex. Here this is done by hand because Jupyter refuses subtraction of lists. One also learns that Jupyter starts the indexing of vectors etc with 0.

```
[7]: p4=[0,2*simplify(hep.fourvec(pf)[1]),2*simplify(hep.
      ↪fourvec(pf)[2]),2*simplify(hep.fourvec(pf)[3])];p4
```

[7]:

$$\left[0, \sqrt{E^2 - M^2} (-\sin(\phi - \theta) + \sin(\phi + \theta)), \sqrt{E^2 - M^2} (\cos(\phi - \theta) - \cos(\phi + \theta)), 2\sqrt{E^2 - M^2} \cos(\theta) \right]$$

```
[8]: tmp=hep.dotprod4(hep.vbu(ki,1,pin,-1),p4)/4/E**2;tmp
```

[8]:

$$\frac{\sqrt{E^2 - M^2} (i \sin(\phi) - \cos(\phi)) \sin(\theta)}{E}$$

```
[9]: t1=tmp.subs(E**2-M**2,P**2);t1
```

[9]:

$$\frac{P (i \sin(\phi) - \cos(\phi)) \sin(\theta)}{E}$$

```
[10]: t1sq=simplify((t1*conjugate(t1)).subs(P**2,E**2-M**2));t1sq
```

[10]:

$$\frac{(E^2 - M^2) \sin^2(\theta)}{E^2}$$

```
[11]: t2=hep.dotprod4(hep.vbu(ki,1,pin,1),p4)/4/E**2;t2
```

[11]:

$$-\frac{m\sqrt{E^2 - M^2} \cos(\theta)}{E^2}$$

The amplitudes may depend on ϕ but the cross section fpr unpolarized beams is independent of ϕ .

```
[12]: t2sq=t2**2;t2sq
```

[12]:

$$\frac{m^2 (E^2 - M^2) \cos^2(\theta)}{E^4}$$

```
[13]: tsqav=simplify((t1sq+t2sq)/2);tsqav
```

[13]:

$$\frac{(E^2 - M^2) (E^2 \sin^2(\theta) + m^2 \cos^2(\theta))}{2E^4}$$

The invariants t, t_0, s expressed in CM variables:

```
[14]: tCM=m**2+M**2-2*E**2+2*sqrt(E**2-m**2)*sqrt(E**2-M**2)*cos(theta);tCM
```

[14]:

$$-2E^2 + M^2 + m^2 + 2\sqrt{E^2 - M^2}\sqrt{E^2 - m^2}\cos(\theta)$$

```
[15]: t0CM=tCM-M**2-m**2;t0CM
```

[15]:

$$-2E^2 + 2\sqrt{E^2 - M^2}\sqrt{E^2 - m^2}\cos(\theta)$$

```
[16]: sCM=4*E**2;sCM
```

[16]:

$$4E^2$$

Guessing from the results of eemumu we try

```
[17]: tsqav_inv=2*(s*m**2-s*t-t0**2)/s**2;tsqav_inv
```

[17]:

$$\frac{2m^2s - 2st - 2t_0^2}{s^2}$$

```
[18]: tsqav_invv1=tsqav_inv.subs(s,sCM)
tsqav_invv2=tsqav_invv1.subs(t,tCM)
tsqav_invv3=tsqav_invv2.subs(t0,t0CM)
proof=simplify(tsqav_invv3-tsqav)
proof
```

[18]:

$$0$$

and prove it. Another useful form is

```
[19]: tsqav_alt=beta**2*sin(theta)**2/2+m**2*beta**2*cos(theta)**2/2/E**2;tsqav_alt
```

[19]:

$$\frac{\beta^2 \sin^2(\theta)}{2} + \frac{\beta^2 m^2 \cos^2(\theta)}{2E^2}$$

```
[20]: simplify(tsqav_alt.subs(beta**2,1-M**2/E**2)-tsqav)
```

[20]:

$$0$$

In contrast to the procedure in the eemumu notebook we here have pions travelling in the θ, ϕ direction produced from positrons and electrons with spins up and down along the x axis. The columns of the transformation matrix yield for $\theta = \pi/2, \phi = 0$

$$|\uparrow\rangle = \frac{1}{\sqrt{2}} (|\frac{1}{2}\rangle + |\frac{-1}{2}\rangle)$$

$$|\downarrow\rangle = \frac{1}{\sqrt{2}} \left(-|\frac{1}{2}\rangle + |\frac{-1}{2}\rangle \right)$$

leading to the helicity states

$$\begin{aligned} |e^+ \uparrow\rangle &= \frac{1}{\sqrt{2}} (|e^+, R\rangle + |e^+, L\rangle) \\ |e^- \downarrow\rangle &= \frac{1}{\sqrt{2}} (-|e^-, L\rangle + |e^-, R\rangle) . \end{aligned}$$

The incoming state is calculated from the product of the helicity states. For $m = 0$ only

$$|e^+ \uparrow\rangle |e^- \downarrow\rangle = \frac{1}{2} (|e^+, L\rangle |e^-, R\rangle - |e^+, R\rangle |e^-, L\rangle)$$

survives. Thus the incoming current has to be calculated from $\bar{v}_L(k_i) \gamma^\mu u_R(p_i) - \bar{v}_R(k_i) \gamma^\mu u_L(p_i)$.

[21]: `hep.vbu(ki,-1,pin,1)`

[21]:

$$[0, -2E, -2iE, 0]$$

[22]: `hep.vbu(ki,1,pin,-1)`

[22]:

$$[0, 2E, -2iE, 0]$$

[23]: `vbudif=[0,-2*E,0,0];vbudif`

[23]:

$$[0, -2E, 0, 0]$$

The calculation of the amplitude is very simple via

[24]: `tmp=simplify(vbudif[1]*p4[1])/4/E**2;tmp`

[24]:

$$-\frac{\sqrt{E^2 - M^2} \sin(\theta) \cos(\phi)}{E}$$

which gives (up to kinematical factors) the polarized cross section after squaring and polishing

[25]: `polstp=tmp**2;polstp`

[25]:

$$\frac{(E^2 - M^2) \sin^2(\theta) \cos^2(\phi)}{E^2}$$

```
[26]: sigP=polsqP.subs(E**2-M**2,E**2*beta**2);sigP
```

[26]:

$$\beta^2 \sin^2(\theta) \cos^2(\phi)$$

which is the result of the standard reference Y.S.Tsai, PRD12, 3533 (1975).
Combining with the unpolarized cross section (next line) we obtain the result for beams with a partial polarization ζ^2

```
[27]: sigU=beta**2*sin(theta)**2/2;sigU
```

[27]:

$$\frac{\beta^2 \sin^2(\theta)}{2}$$

```
[28]: (1-xi**2)*sigU+xi**2*sigP
```

[28]:

$$\beta^2 \zeta^2 \sin^2(\theta) \cos^2(\phi) + \frac{\beta^2 (-\zeta^2 + 1) \sin^2(\theta)}{2}$$

```
[29]: sig=sigU-(xi**2*beta**2*sin(theta)**2*cos(2*phi))/2;sig
```

[29]:

$$-\frac{\beta^2 \zeta^2 \sin^2(\theta) \cos(2\phi)}{2} + \frac{\beta^2 \sin^2(\theta)}{2}$$

and finally after conventionally switching to a magnetic field along the y axis the cross section $d\sigma/d\Omega$

```
[30]: dsigdOm=simplify(alpha**2/16/E**2*sig);print('dsigma/dOmega='); dsigdOm
```

dsigma/dOmega=

[30]:

$$\frac{\alpha^2 \beta^2 (-\zeta^2 \cos(2\phi) + 1) \sin^2(\theta)}{32E^2}$$

The amplitudes squared for $e\pi$ scattering is obtained via crossing $s \leftrightarrow t$ with a minus sign because only one fermion line is crossed

```
[31]: tsqav_sc=-2*(t*m**2-s*t-s0**2)/t**2;tsqav_sc
```

[31]:

$$\frac{-2m^2 t + 2st + 2s_0^2}{t^2}$$

```
[32]: dsgdt=16*pi**2*alpha**2/(16*pi*s0**2*(1-4*m**2*M**2/s0**2))*tsqav_sc;
      ↪print('dsigma/dt='); dsgdt
```

dsigma/dt=

[32]:

$$\frac{\pi\alpha^2(-2m^2t+2st+2s_0^2)}{s_0^2t^2\left(-\frac{4M^2m^2}{s_0^2}+1\right)}$$

The Mott cross section is obtained in the limit $M \rightarrow \infty$. It is identical to the result of eemumu notebook. The basic difference between pions and protons is the magnetic moment of the proton which is proportional to $1/M$.

[]: